most instructions except memory related

otbn_model/spec/vt_ops.dfy
@@ -66,12 +66,12 @@ module vt_ops {
 
     datatype fgroups_t = fgroups_t(fg0: flags_t, fg1: flags_t)
 
-    function select_fgroup(fgps: fgroups_t, which: uint1): flags_t
+    function method select_fgroup(fgps: fgroups_t, which: uint1): flags_t
     {
         if which == 0 then fgps.fg0 else fgps.fg1
     }
 
-    function get_flag(fgps: fgroups_t, which_group: uint1, which_flag: uint2) : bool
+    function method get_flag(fgps: fgroups_t, which_group: uint1, which_flag: uint2) : bool
     {
         if which_flag == 0 then select_fgroup(fgps, which_group).cf 
         else if which_flag == 1 then select_fgroup(fgps, which_group).msb
@@ -79,9 +79,9 @@ module vt_ops {
         else select_fgroup(fgps, which_group).zero
     }
 
-    function update_fgroups(fgps: fgroups_t, which_group: uint1, new_flags_t: flags_t) : fgroups_t
+    function method update_fgroups(fgps: fgroups_t, which_group: uint1, new_flags: flags_t) : fgroups_t
     {
-        if which_group == 0 then fgps.(fg0 := new_flags_t) else fgps.(fg1 := new_flags_t)
+        if which_group == 0 then fgps.(fg0 := new_flags) else fgps.(fg1 := new_flags)
     }
 
 /* memory definions */
@@ -146,104 +146,28 @@ module vt_ops {
         && iter.index < |iter.buff|
     }
 
-/* state definions */
+/* stateless semantic functions  */
 
-    datatype state = state(
-        gprs: gprs_t, // 32-bit registers
-        wdrs: wdrs_t, // 256-bit registers
-
-        wmod: uint256,
-        wrnd: uint256,
-        wacc: uint256,
-
-        fgroups: fgroups_t,
-
-        xmem: xmem_t,
-        wmem: wmem_t,
-
-        ok: bool)
+    function method set_flags(carry: uint1, value: uint256): flags_t
     {
-        function eval_reg32(r: reg32_t) : uint32
-        {
-            if r.index == 0 then 0
-            else gprs[r.index]
-        }
-
-        function eval_reg256(r: reg256_t) : uint256
-        {
-            match r {
-                case WDR(index) => wdrs[r.index]
-                case WMOD => wmod
-                case WRND => wrnd
-                case WACC => wacc
-            }
-        }
-
-        function write_reg32(r: reg32_t, v: uint32) : state
-        {
-            if r.index == 0 then this
-            else this.(gprs := gprs[r.index := v])
-        }
-
-        function eval_ADD(xrd: reg32_t, xrs1: reg32_t, xrs2: reg32_t): state
-        {
-            var v1 := eval_reg32(xrs1);
-            var v2 := eval_reg32(xrs2);
-            var sum := uint32_add(v1, v2);
-            write_reg32(xrd, sum)
-        }
-        
-        function eval_ADDI(xrd: reg32_t, xrs1: reg32_t, imm: uint32): state
-        {
-            var v1 := eval_reg32(xrs1);
-            var sum := uint32_add(v1, imm);
-            write_reg32(xrd, sum)
-        }
-
-        function eval_LUI(xrd: reg32_t, imm: uint32)
+        flags_t(carry == 1, uint256_msb(value) == 1, uint256_lsb(value) == 1, value == 0)
     }
 
-    predicate valid_state(s: state)
-    {
-        s.ok
-    }
-
-    /* semantics definions (THESE ARE NOT CONNECTED TO BELOW YET) */
-
-    function otbn_addc(x: uint256, y: uint256, shift: shift_t, carry: bool) : (uint256, flags_t)
+    function method otbn_addc(x: uint256, y: uint256, shift: shift_t, carry: bool) : (uint256, flags_t)
     {
         var cin := if carry then 1 else 0;
         var (sum, cout) := uint256_addc(x, uint256_sb(y, shift), cin);
-        // TODO: MSB/LSB
-        var fg := flags_t(cout == 1, false, false, sum == 0);
-        (sum, fg)
+        (sum, set_flags(cout, sum))
     }
 
-    // function otbn_addm(x: uint256, y: uint256, mod: uint256) : uint256
-    // {
-    //     var (sum, _) := otbn_add_carray(x, y, false);
-    //     if sum >= mod then sum - mod else sum
-    // }
-
-    function otbn_subb(x: uint256, y: uint256, shift: shift_t, borrow: bool) : (uint256, flags_t)
+    function method otbn_subb(x: uint256, y: uint256, shift: shift_t, borrow: bool) : (uint256, flags_t)
     {
         var cf := if borrow then 1 else 0;
         var (diff, cout) := uint256_subb(x, uint256_sb(y, shift), cf);
-        // TODO: MSB/LSB
-        var fg := flags_t(cout == 1, false, false, diff == 0);
-        (diff, fg)
+        (diff, set_flags(cout, diff))
     }
 
-    function otbn_subm(x: uint256, y: uint256, wmod: uint256) : uint256
-        requires false;
-    {
-    //     // FIXME: some bound checking?
-    //     // assume false;
-        var result := (x as bv256 - y as bv256) as uint256;
-        if result >= wmod then (result as bv256 - wmod as bv256) as uint256 else result
-    }
-
-    function otbn_mulqacc(
+    function method otbn_mulqacc(
         zero: bool,
         x: uint256, qx: uint2,
         y: uint256, qy: uint2,
@@ -290,79 +214,274 @@ module vt_ops {
         else x * BASE_192
     }
 
-    function otbn_xor(x: uint256, y: uint256, shift: shift_t) : uint256
+    function method otbn_xor(x: uint256, y: uint256, shift: shift_t, carry: bool): (uint256, flags_t)
     {
-        uint256_xor(x, uint256_sb(y, shift))
+        var result := uint256_xor(x, uint256_sb(y, shift));
+        // keep the old carry
+        (result, set_flags(bool_to_uint1(carry), result))
     }
 
-    function otbn_or(x: uint256, y: uint256, shift: shift_t) : uint256
+    function method otbn_sel(x: uint256, y: uint256, sel: bool): uint256
     {
-        uint256_or(x, uint256_sb(y, shift))
-    }
-            
-    function otbn_and(x: uint256, y: uint256, shift: shift_t) : uint256
-    {
-        uint256_and(x, uint256_sb(y, shift))
+        if sel then x else y
     }
 
-    function otbn_rshi(x: uint256, y: uint256, shift_amt: int) : uint256
-        requires 0 <= shift_amt < 256;
+/* state definions */
+
+    predicate method admissible_xmem_addr(addr: uint32)
     {
-        var concat : int := x * BASE_256 + y;
-        (concat / pow2(shift_amt)) % BASE_256
+        && addr % 4 == 0
+        && addr < DMEM_LIMIT
+    }
+
+    datatype state = state(
+        gprs: gprs_t, // 32-bit registers
+        wdrs: wdrs_t, // 256-bit registers
+
+        wmod: uint256,
+        wrnd: uint256,
+        wacc: uint256,
+
+        fgroups: fgroups_t,
+
+        xmem: xmem_t,
+        wmem: wmem_t,
+
+        ok: bool)
+    {
+        function method read_reg32(r: reg32_t): uint32
+        {
+            if r.index == 0 then 0
+            else gprs[r.index]
+        }
+
+        function method write_reg32(r: reg32_t, v: uint32): state
+        {
+            if r.index == 0 then this
+            else this.(gprs := gprs[r.index := v])
+        }
+
+        function method read_xmem(addr: uint32): uint32
+            requires admissible_xmem_addr(addr)
+        {
+            if addr in xmem then xmem[addr] else 0
+        }
+
+        function method write_xmem(addr: uint32, v: uint32): state
+            requires admissible_xmem_addr(addr)
+        {
+            this.(xmem := xmem[addr := v])
+        }
+
+        function method eval_ADD(xrd: reg32_t, xrs1: reg32_t, xrs2: reg32_t): state
+        {
+            var v1 := read_reg32(xrs1);
+            var v2 := read_reg32(xrs2);
+            var sum := uint32_add(v1, v2);
+            write_reg32(xrd, sum)
+        }
+
+        function method eval_ADDI(xrd: reg32_t, xrs1: reg32_t, imm: imm12): state
+            requires imm > 0
+        {
+            var v1 := read_reg32(xrs1);
+            var sum := uint32_add(v1, imm);
+            write_reg32(xrd, sum)
+        }
+
+        function method eval_LW(xrs1: reg32_t, xrs2: reg32_t, offset: imm12): state
+            requires offset > 0
+        {
+            var addr := uint32_add(read_reg32(xrs1), offset);
+            if !admissible_xmem_addr(addr) then this.(ok := false)
+            else write_xmem(addr, read_reg32(xrs2))
+        }
+
+        function method eval_SW(xrd: reg32_t, xrs1: reg32_t, offset: imm12): state
+            requires offset > 0
+        {
+            var addr := uint32_add(read_reg32(xrs1), offset);
+            if !admissible_xmem_addr(addr) then this.(ok := false)
+            else write_reg32(xrd, read_xmem(addr))
+        }
+
+        function method eval_LI(xrd: reg32_t, imm: uint32): state
+        {
+            write_reg32(xrd, imm)
+        }
+
+        function method read_reg256(r: reg256_t) : uint256
+        {
+            match r {
+                case WDR(index) => wdrs[r.index]
+                case WMOD => wmod
+                case WRND => wrnd
+                case WACC => wacc
+            }
+        }
+
+        function method write_reg256(r: reg256_t, v: uint256): state
+        {
+            match r {
+                case WDR(index) => this.(wdrs := wdrs[r.index := v])
+                case WMOD => this.(wmod := v)
+                case WRND => this.(wrnd := v)
+                case WACC => this.(wacc := v)
+            }
+        }
+
+        function method read_flag(which_group: uint1, which_flag: uint2): bool
+        {
+            get_flag(fgroups, which_group, which_flag)
+        }
+
+        function method write_flags(which_group: uint1, new_flags: flags_t): state
+        {
+            this.(fgroups := update_fgroups(fgroups, which_group, new_flags))
+        }
+
+        function method eval_BN_ADD(wrd: reg256_t, wrs1: reg256_t, wrs2: 
+        reg256_t, shift: shift_t, fg: uint1): state
+        {
+            var v1 := read_reg256(wrs1);
+            var v2 := read_reg256(wrs2);
+            var (sum, flags) := otbn_addc(v1, v2, shift, false);
+            write_reg256(wrd, sum).write_flags(fg, flags)
+        }
+
+        function method eval_BN_ADDC(wrd: reg256_t, wrs1: reg256_t, wrs2: reg256_t, shift: shift_t, fg: uint1): state
+        {
+            var v1 := read_reg256(wrs1);
+            var v2 := read_reg256(wrs2);
+            var carry := read_flag(fg, 0);
+            var (sum, flags) := otbn_addc(v1, v2, shift, carry);
+            write_reg256(wrd, sum).write_flags(fg, flags)
+        }
+
+        function method eval_BN_ADDI(wrd: reg256_t, wrs1: reg256_t, imm: uint10, fg: uint1): state
+        {
+            var v1 := read_reg256(wrs1);
+            var (sum, flags) := otbn_addc(v1, imm, SFT_DFT, false);
+            write_reg256(wrd, sum).write_flags(fg, flags)
+        }
+
+        function method eval_BN_MULQACC(zero: bool, wrs1: reg256_t, qwsel1: uint2, wrs2: reg256_t, qwsel2: uint2, shift_qws: uint2): state
+        {
+            var v1 := read_reg256(wrs1);
+            var v2 := read_reg256(wrs2);
+            var v3 := read_reg256(WACC);
+            var product := otbn_mulqacc(zero, v1, qwsel1, v2, qwsel2, shift_qws, v3);
+            write_reg256(WACC, product)
+        }
+        
+        function method eval_BN_MULQACC_SO(zero: bool, wrd: reg256_t, lower: bool, wrs1: reg256_t, qwsel1: uint2, wrs2: reg256_t, qwsel2: uint2, shift_qws: uint2): state
+        {
+            var v1 := read_reg256(wrs1);
+            var v2 := read_reg256(wrs2);
+            var v3 := read_reg256(WACC);
+            var v4 := read_reg256(wrd);
+            var product := otbn_mulqacc(zero, v1, qwsel1, v2, qwsel2, shift_qws, v3);
+            var lh, uh := uint256_lh(product), uint256_uh(product);
+            // the upper half stay in wacc
+            write_reg256(WACC, uh).
+            // the lower half gets written back into dst
+            write_reg256(wrd, uint256_hwb(v4, lh, lower))
+        }
+
+        function method eval_BN_SUB(wrd: reg256_t, wrs1: reg256_t, wrs2: reg256_t, shift: shift_t, fg: uint1): state
+        {
+            var v1 := read_reg256(wrs1);
+            var v2 := read_reg256(wrs2);
+            var (diff, flags) := otbn_subb(v1, v2, shift, false);
+            write_reg256(wrd, diff).write_flags(fg, flags)
+        }
+        
+        function method eval_BN_SUBB(wrd: reg256_t, wrs1: reg256_t, wrs2: reg256_t, shift: shift_t, fg: uint1): state
+        {
+            var v1 := read_reg256(wrs1);
+            var v2 := read_reg256(wrs2);
+            var borrow := read_flag(fg, 0);
+            var (diff, flags) := otbn_subb(v1, v2, shift, borrow);
+            write_reg256(wrd, diff).write_flags(fg, flags)
+        }
+
+        function method eval_BN_XOR(wrd: reg256_t, wrs1: reg256_t, wrs2: reg256_t, shift: shift_t, fg: uint1): state
+        {
+            var v1 := read_reg256(wrs1);
+            var v2 := read_reg256(wrs2);
+            var carry := read_flag(fg, 0);
+            var (result, flags) := otbn_xor(v1, v2, shift, carry);
+            write_reg256(wrd, result).write_flags(fg, flags)
+        }
+
+        function method eval_BN_SEL(wrd: reg256_t, wrs1: reg256_t, wrs2: reg256_t, fg: uint1, flag: uint2): state
+        {
+            var v1 := read_reg256(wrs1);
+            var v2 := read_reg256(wrs2);
+            var sel := read_flag(fg, flag);
+            var result := otbn_sel(v1, v2, sel);
+            write_reg256(wrd, result)
+        }
+
+        function method eval_BN_MOV(wrd: reg256_t, wrs: reg256_t): state
+        {
+            write_reg256(wrd, read_reg256(wrs))
+        }
+
+        function method eval_BN_MOVR(grd: reg32_t, grd_inc: bool, grs: reg32_t, grs_inc: bool): state
+        {
+            var di := read_reg32(grd);
+            var si := read_reg32(grs);
+            if di > 5 || si > 5 then 
+                this.(ok := false)
+            else
+                write_reg32(grd, if grd_inc then di + 1 else di).
+                write_reg32(grs, if grs_inc then di + 1 else si).
+                write_reg256(WDR(di), read_reg256(WDR(si)))
+        }
+    }
+
+    predicate valid_state(s: state)
+    {
+        s.ok
     }
 
 /* instruction definions (THESE ARE NOT CONNECTED TO ABOVE YET) */
 
     datatype ins32 =
         | ADD(xrd: reg32_t, xrs1: reg32_t, xrs2: reg32_t)
-        | ADDI(xrd: reg32_t, xrs1: reg32_t, imm: uint32)
-        | LUI(xrd: reg32_t, imm: uint32)
-        | SUB(xrd: reg32_t, xrs1: reg32_t, xrs2: reg32_t)
-        | AND(xrd: reg32_t, xrs1: reg32_t, xrs2: reg32_t)
-        | ANDI(xrd: reg32_t, xrs1: reg32_t, imm: uint32)
-        | OR(xrd: reg32_t, xrs1: reg32_t, xrs2: reg32_t)
-        | ORI(xrd: reg32_t, xrs1: reg32_t, imm: uint32)
-        | XOR(xrd: reg32_t, xrs1: reg32_t, xrs2: reg32_t)
-        | XORI(xrd: reg32_t, xrs1: reg32_t, imm: uint32)
-        | LW(xrd: reg32_t, xrs1: reg32_t, imm: uint32)
-        | SW(xrs1: reg32_t, xrs2: reg32_t, imm: uint32)
-        | BEQ(xrs1: reg32_t, xrs2: reg32_t, offset: uint32)
-        | BNE(xrs1: reg32_t, xrs2: reg32_t, offset: uint32)
+        | ADDI(xrd: reg32_t, xrs1: reg32_t, imm: imm12)
+        | LW(xrd: reg32_t, xrs1: reg32_t, offset: imm12)
+        | SW(xrs1: reg32_t, xrs2: reg32_t, offset: imm12)
         | LOOP(grs: reg32_t, bodysize: uint32)
         | LOOPI(iterations: uint32, bodysize: uint32)
-        | JAL(xrd: reg32_t, offset: uint32)
-        | JALR(xrd: reg32_t, xrs1: reg32_t, offset: uint32)
-        | CSRRS(xrd: reg32_t, csr: reg32_t, xrs2: reg32_t)
-        | CSRRW(xrd: reg32_t, csr: reg32_t, xrs2: reg32_t)
-        | ECALL // TODO
-        | LI(xrd: reg32_t, imm: uint32)
+        | LI(xrd: reg32_t, imm32: uint32)
 
     datatype ins256 =
         | BN_ADD(wrd: reg256_t, wrs1: reg256_t, wrs2: reg256_t, shift: shift_t, fg: uint1)
         | BN_ADDC(wrd: reg256_t, wrs1: reg256_t, wrs2: reg256_t, shift: shift_t, fg: uint1)
-        | BN_ADDI(wrd: reg256_t, wrs1: reg256_t, imm: uint256, fg: uint1)
-        | BN_ADDM(wrd: reg256_t, wrs1: reg256_t, wrs2: reg256_t)
-        | BN_MULQACC(zero: bool, wrs1: reg256_t, qwsel1: uint32, wrs2: reg256_t, qwsel2: uint32, shift_qws: uint2)
-        | BN_MULQACC_SO(zero: bool, wrd: reg256_t, lower: bool, wrs1: reg256_t, qwsel1: uint32, wrs2: reg256_t, qwsel2: uint32, shift_qws: uint2)
+        | BN_ADDI(wrd: reg256_t, wrs1: reg256_t, imm: uint10, fg: uint1)
+        // | BN_ADDM(wrd: reg256_t, wrs1: reg256_t, wrs2: reg256_t)
+        | BN_MULQACC(zero: bool, wrs1: reg256_t, qwsel1: uint2, wrs2: reg256_t, qwsel2: uint2, shift_qws: uint2)
+        | BN_MULQACC_SO(zero: bool, wrd: reg256_t, lower: bool, wrs1: reg256_t, qwsel1: uint2, wrs2: reg256_t, qwsel2: uint2, shift_qws: uint2)
         | BN_SUB(wrd: reg256_t, wrs1: reg256_t, wrs2: reg256_t, shift: shift_t, fg: uint1)
         | BN_SUBB(wrd: reg256_t, wrs1: reg256_t, wrs2: reg256_t, shift: shift_t, fg: uint1)
-        | BN_SUBI(wrd: reg256_t, wrs1: reg256_t, imm: uint256, fg: uint1)
-        | BN_SUBM(wrd: reg256_t, wrs1: reg256_t, wrs2: reg256_t)
-        | BN_AND(wrd: reg256_t, wrs1: reg256_t, wrs2: reg256_t, shift: shift_t)
-        | BN_OR(wrd: reg256_t, wrs1: reg256_t, wrs2: reg256_t, shift: shift_t)
-        | BN_NOT(wrd: reg256_t, wrs1: reg256_t, wrs2: reg256_t, shift: shift_t)
-        | BN_XOR(wrd: reg256_t, wrs1: reg256_t, wrs2: reg256_t, shift: shift_t)
-        | BN_RSHI(wrd: reg256_t, wrs1: reg256_t, wrs2: reg256_t, imm: uint256)
-        | BN_SEL(wrd: reg256_t, wrs1: reg256_t, wrs2: reg256_t, fg: uint1, flag:uint2)
-        | BN_CMP(wrs1: reg256_t, wrs2: reg256_t, fg: uint1)
-        | BN_CMPB(wrs1: reg256_t, wrs2: reg256_t, fg: uint1)
+        // | BN_SUBI(wrd: reg256_t, wrs1: reg256_t, imm: uint10, fg: uint1)
+        // | BN_SUBM(wrd: reg256_t, wrs1: reg256_t, wrs2: reg256_t)
+        // | BN_AND(wrd: reg256_t, wrs1: reg256_t, wrs2: reg256_t, shift: shift_t, fg: uint1)
+        // | BN_OR(wrd: reg256_t, wrs1: reg256_t, wrs2: reg256_t, shift: shift_t, fg: uint1)
+        // | BN_NOT(wrd: reg256_t, wrs1: reg256_t, wrs2: reg256_t, shift: shift_t, fg: uint1)
+        | BN_XOR(wrd: reg256_t, wrs1: reg256_t, wrs2: reg256_t, shift: shift_t, fg: uint1)
+        // | BN_RSHI(wrd: reg256_t, wrs1: reg256_t, wrs2: reg256_t, imm: uint256)
+        | BN_SEL(wrd: reg256_t, wrs1: reg256_t, wrs2: reg256_t, fg: uint1, flag: uint2)
+        // | BN_CMP(wrs1: reg256_t, wrs2: reg256_t, fg: uint1)
+        // | BN_CMPB(wrs1: reg256_t, wrs2: reg256_t, fg: uint1)
         | BN_LID(grd: reg32_t, grd_inc: bool, offset: uint32, grs: reg32_t, grs_inc: bool)
         | BN_SID(grs2: reg32_t, grs2_inc: bool, offset: uint32, grs1: reg32_t, grs1_inc: bool)
         | BN_MOV(wrd: reg256_t, wrs: reg256_t)
         | BN_MOVR(grd: reg32_t, grd_inc: bool, grs: reg32_t, grs_inc: bool)
-        | BN_WSRRS // TODO
-        | BN_WSRRW // TODO
+        // | BN_WSRRS 
+        // | BN_WSRRW
 
 
     predicate eval_ins32(xins: ins32, s: state, r: state)
@@ -409,7 +528,7 @@ module vt_ops {
     function eval_cond(s: state, wc: whileCond): nat
     {
         match wc 
-            case RegCond(r) => s.eval_reg32(r)
+            case RegCond(r) => s.read_reg32(r)
             case ImmCond(c) => c
     }
 
