otbn_model/spec/bv_ops.dfy
@@ -18,7 +18,8 @@ module bv_ops {
     type uint256 = i :int | 0 <= i < BASE_256
     type uint512 = i :int | 0 <= i < BASE_512
 
-    type int12     = i :int | -2048 <= i <= 2047
+    type imm12   = i :int | -2048 <= i <= 2047
+    type uint10  = i :int | 0 <= i < 1024
 
     datatype shift_t = SFT(left: bool, bytes: uint5)
 
@@ -34,7 +35,7 @@ module bv_ops {
         power(BASE_256, e)
     }
 
-    function bool_to_uint1(i:bool) : uint1
+    function method bool_to_uint1(i:bool) : uint1
     {
         if i then 1 else 0
     }
@@ -85,14 +86,9 @@ module bv_ops {
         (x - y) % BASE_32
     }
 
-    function {:extern} uint32_se(x:uint32, size:int):uint32
-    //     requires 0 < size < 32;
-  // {
-  //   var sign : bv32 := (x as bv32 >> (size - 1));
-  //   var ext := if sign == 0 then 0 else (sign << (32 - (size + 1))) - 1;
-  //   (x as bv32 | ext) as uint32
-  //   
-  // }
+    function method uint256_msb(x: uint256): uint1
+
+    function method uint256_lsb(x: uint256): uint1
 
     function method uint256_mul(x: uint256, y: uint256): uint256
     {
@@ -138,16 +134,16 @@ module bv_ops {
         (x as bv256 | y as bv256) as uint256
     }
 
-    function {:extern} {:opaque} uint256_ls(x: uint256, num_bytes: uint5): (r: uint256)
+    function method uint256_ls(x: uint256, num_bytes: uint5): (r: uint256)
         ensures (num_bytes == 8 && x < BASE_192) ==> (r == x * BASE_64);
     // {
     //     //assume false;
     //     (x as bv256 << (num_bytes * 8)) as uint256
     // }
 
-    function {:extern} {:opaque} uint256_rs(x: uint256, num_bytes: uint5): uint256
+    function method uint256_rs(x: uint256, num_bytes: uint5): uint256
 
-    function uint256_sb(b: uint256, shift: shift_t) : uint256
+    function method uint256_sb(b: uint256, shift: shift_t) : uint256
     {    
         var count := shift.bytes;
         if count == 0 then b
@@ -237,7 +233,7 @@ module bv_ops {
     }
 
     function method {:opaque} uint256_qsel(x: uint256, qx: uint2): uint64
-        {
+    {
         if qx == 0 then
             uint256_lh(x) % BASE_64
         else if qx == 1 then
